Properly define Y combinator tree
- replace with unicode where possible
- make `Var` explicit
- add `bfvar` to group both free and bound variables
- add abstractions and variable to `hnf` case of `BöhmTree`

src/Bohm_Tree.lean
@@ -13,20 +13,20 @@ variable {Var : Type u}
 
 inductive isHeadRedexApp : Term Var → Prop where
   | base N P₁ : isHeadRedexApp ((Term.abs N).app P₁)
-  | step T Pₙ : isHeadRedexApp T -> isHeadRedexApp (T.app Pₙ)
+  | step T Pₙ : isHeadRedexApp T → isHeadRedexApp (T.app Pₙ)
 
 inductive isHeadRedex : Term Var → Prop where
-  | base T : isHeadRedexApp T -> isHeadRedex T
-  | step T : isHeadRedex T -> isHeadRedex (Term.abs T)
+  | base T : isHeadRedexApp T → isHeadRedex T
+  | step T : isHeadRedex T → isHeadRedex (Term.abs T)
 
 inductive isHeadNormalApp : Term Var → Prop where
   | base_free y : isHeadNormalApp (Term.fvar y)
   | base_bound n : isHeadNormalApp (Term.bvar n)
-  | step T Pₙ : isHeadNormalApp T -> isHeadNormalApp (T.app Pₙ)
+  | step T Pₙ : isHeadNormalApp T → isHeadNormalApp (T.app Pₙ)
 
 inductive isHeadNormal : Term Var → Prop where
-  | base T : isHeadNormalApp T -> isHeadNormal T
-  | step T : isHeadNormal T -> isHeadNormal (Term.abs T)
+  | base T : isHeadNormalApp T → isHeadNormal T
+  | step T : isHeadNormal T → isHeadNormal (Term.abs T)
 
 -- Lemma 3.2
 lemma normal_or_redex (T : Term Var) : isHeadRedex T ∨ isHeadNormal T := by
@@ -60,49 +60,72 @@ inductive List.BetaEquiv : List (Term Var) → List (Term Var) → Prop where
   | base : [].BetaEquiv []
   | step as bs T₁ T₂ : T₁.BetaEquiv T₂ → as.BetaEquiv bs → (T₁ :: as).BetaEquiv (T₂ :: bs)
 
+def bfvar (Var : Type u) := { v : Term Var // (exists n, v = Term.bvar n) ∨ (exists v', v = Term.fvar v') }
+
 -- Reduction does not affect the number of leading abstractions, the head variable, or the number of arguments of the head-variable
-lemma reduction_preservation (n m : ℕ) (y z : Var) (Ps Qs : List (Term Var)) :
-    (nfoldAbs n (nfoldApp Ps (Term.fvar y))).Beta (nfoldAbs m (nfoldApp Qs (Term.fvar z))) ->
+lemma reduction_preservation_fvar (n m : ℕ) (y z : bfvar Var) (Ps Qs : List (Term Var)) :
+    (nfoldAbs n (nfoldApp Ps y.val)).Beta (nfoldAbs m (nfoldApp Qs z.val)) →
     n = m ∧ y = z ∧ Ps.BetaEquiv Qs := by
   sorry
 
 -- Lemma 3.5
-lemma hnfs_similar (n m : ℕ) (y z : Var) (Ps Qs : List (Term Var)) (M : Term Var) :
-    M.BetaEquiv (nfoldAbs n (nfoldApp Ps (Term.fvar y))) ->
-    M.BetaEquiv (nfoldAbs m (nfoldApp Qs (Term.fvar z))) ->
+lemma hnfs_similar_fvar (n m : ℕ) (y z : bfvar Var) (Ps Qs : List (Term Var)) (M : Term Var) :
+    M.BetaEquiv (nfoldAbs n (nfoldApp Ps y.val)) →
+    M.BetaEquiv (nfoldAbs m (nfoldApp Qs z.val)) →
     n = m ∧ y = z ∧ Ps.BetaEquiv Qs := by
   sorry
 
-inductive BöhmTreeF (T : Type u) : Type u where
+inductive BöhmTreeF (Var : Type u) (T : Type u) : Type u where
   | no_hnf
-  | hnf (n : ℕ) (branches : Fin n → T)
+  | hnf (n : ℕ) (num_abstractions : ℕ) (v : bfvar Var) (branches : ULift (Fin n) → T)
 
-instance : Inhabited (BöhmTreeF PUnit) where default := .no_hnf
+instance : Inhabited (BöhmTreeF Var PUnit) where default := .no_hnf
 
 inductive BöhmTreeF.in : Type u where
   | no_hnf
-  | hnf (n : ℕ)
+  | hnf (n : ℕ) (num_abstractions : ℕ) (v : bfvar Var)
 
-instance : PF BöhmTreeF where
+instance : PF (BöhmTreeF Var) where
   P := ⟨BöhmTreeF.in, fun
     | .no_hnf => PEmpty
-    | .hnf n => Fin n⟩
+    | .hnf n na v => ULift (Fin n)⟩
   unpack
     | .no_hnf => .obj (.no_hnf) nofun
-    | .hnf n f => .obj (.hnf n) f
+    | .hnf n na v f => .obj (.hnf n na v) f
   pack
     | .obj (.no_hnf) _ => .no_hnf
-    | .obj (.hnf n) f => .hnf n f
+    | .obj (.hnf n na v) f => .hnf n na v f
   unpack_pack := by rintro _ ⟨⟩ <;> simp
   pack_unpack := by rintro _ (⟨⟨⟩, _⟩ | ⟨⟨⟩⟩) <;> simp ; funext x ; cases x
 
-abbrev BöhmTree := CoInd BöhmTreeF
-abbrev BöhmTreeN (n : Nat) : Type u := CoIndN BöhmTreeF n
+abbrev BöhmTree (Var : Type u) := CoInd (BöhmTreeF Var)
+abbrev BöhmTreeN (Var : Type u) (n : Nat) : Type u := CoIndN (BöhmTreeF Var) n
 
-def BöhmTree.fold (t : BöhmTreeF BöhmTree) : BöhmTree := CoInd.fold _ t
-def BöhmTree.unfold (t : BöhmTree) : BöhmTreeF BöhmTree := CoInd.unfold _ t
-def BöhmTree.no_hnf : BöhmTree := BöhmTree.fold .no_hnf
-def BöhmTree.hnf (n : ℕ) (f : Fin n → BöhmTree) : BöhmTree := BöhmTree.fold (.hnf n f)
+def BöhmTree.fold (t : (BöhmTreeF Var) (BöhmTree Var)) : (BöhmTree Var) := CoInd.fold _ t
+def BöhmTree.unfold (t : (BöhmTree Var)) : (BöhmTreeF Var) (BöhmTree Var) := CoInd.unfold _ t
+def BöhmTree.no_hnf : (BöhmTree Var) := BöhmTree.fold .no_hnf
+def BöhmTree.hnf (n : ℕ) (na : ℕ) (t : bfvar Var) (f : ULift (Fin n) → (BöhmTree Var)) : (BöhmTree Var) := BöhmTree.fold (.hnf n na t f)
+
+def hasAsHnf : Term Var → (n : ℕ) → List (Term Var) → bfvar Var → Prop := λ T n Ps y ↦
+  let T' := nfoldAbs n (nfoldApp Ps y.val) ; isHeadNormal T' ∧ T.BetaEquiv T'
 
 -- Definition 3.7
-def BT : Term Var → BöhmTree := sorry
+coinductive BT (Var : Type u) : Term Var → BöhmTree Var → Prop where
+  | no_hnf (T : Term Var) :
+      ¬(exists n Ps y, hasAsHnf T n Ps y) →
+      BT Var T BöhmTree.no_hnf
+  | hnf_fvar (T : Term Var) (n : ℕ) (na : ℕ) (t : bfvar Var) (Ps : Vector (Term Var) n) (y : bfvar Var) (Ts : ULift (Fin n) → BöhmTree Var) :
+      hasAsHnf T n Ps.toList y →
+      forall (m : ULift (Fin n)), BT Var (Ps.get m.down) (Ts m) →
+      BT Var T (BöhmTree.hnf n na t Ts)
+
+--                        λ x .                f      (           x                 x )
+def omega_f : Term Var := Term.abs ((Term.bvar 1).app ((Term.bvar 0).app (Term.bvar 0)))
+--                            λ f .                f      (ωf          ωf     )
+def Ycombinator : Term Var := Term.abs ((Term.bvar 0).app (omega_f.app omega_f))
+
+coinductive is_inf_Ytree : BöhmTree Var → Prop where
+  | Is_inf_Ytree T : is_inf_Ytree T → is_inf_Ytree (BöhmTree.hnf 1 0 ⟨Term.bvar 0, by simp⟩ (λ _ ↦ T))
+
+lemma Ycombinator_tree T : is_inf_Ytree T → BT Var Ycombinator (BöhmTree.hnf 1 1 ⟨Term.bvar 0, by simp⟩ (λ _ ↦ T)) := by
+  sorry
